src/Crypto/AESEncryption.dfy
@@ -8,8 +8,8 @@ module {:extern "AESEncryption"} AESEncryption {
   import opened UInt = StandardLibrary.UInt
 
   export
-    provides AESDecrypt, AESEncrypt, EncryptionSuites, StandardLibrary, UInt, PlaintextDecryptedWithAAD, EncryptionOutputEncryptedWithAAD
-    provides DecryptMock, EncryptMock
+    provides AESDecryptWrapper, AESEncryptWrapper, AESDecrypt, AESEncrypt, EncryptionSuites, StandardLibrary, UInt, PlaintextDecryptedWithAAD, EncryptionOutputEncryptedWithAAD
+    provides IsEncrypted
     reveals EncryptionOutput
 
   datatype EncryptionOutput = EncryptionOutput(cipherText: seq<uint8>, authTag: seq<uint8>)
@@ -19,6 +19,7 @@ module {:extern "AESEncryption"} AESEncryption {
   // in order to ensure that the AAD used is as expected.
   predicate {:axiom} PlaintextDecryptedWithAAD(plaintext: seq<uint8>, aad: seq<uint8>)
   predicate {:axiom} EncryptionOutputEncryptedWithAAD(ciphertext: EncryptionOutput, aad: seq<uint8>)
+  predicate {:axiom} IsEncrypted (ciphertext: seq<uint8>, plaintext: seq<uint8>)
 
   function method EncryptionOutputFromByteSeq(s: seq<uint8>, encAlg: EncryptionSuites.EncryptionSuite): (encArt: EncryptionOutput)
     requires encAlg.Valid()
@@ -29,14 +30,17 @@ module {:extern "AESEncryption"} AESEncryption {
     EncryptionOutput(s[.. |s| - encAlg.tagLen as int], s[|s| - encAlg.tagLen as int ..])
   }
 
-  function DecryptMock (input: seq<uint8>):  (output: seq<uint8>)
-    ensures |input| == |output|
-  
-  function EncryptMock (input: seq<uint8>):  (output: seq<uint8>)
-    ensures DecryptMock(EncryptMock(input)) == input;
-    ensures |input| == |output|
-
   method {:extern "AESEncryption.AES_GCM", "AESEncrypt"} AESEncrypt(encAlg: EncryptionSuites.EncryptionSuite, iv: seq<uint8>, key: seq<uint8>, msg: seq<uint8>, aad: seq<uint8>)
+      returns (res : Result<EncryptionOutput>)
+    requires encAlg.Valid()
+    requires encAlg.alg.AES?
+    requires encAlg.alg.mode.GCM?
+    requires |iv| == encAlg.ivLen as int
+    requires |key| == encAlg.keyLen as int
+    ensures res.Success? ==> EncryptionOutputEncryptedWithAAD(res.value, aad)
+    ensures res.Success? ==> IsEncrypted(res.value.cipherText, msg)
+
+  method AESEncryptWrapper(encAlg: EncryptionSuites.EncryptionSuite, iv: seq<uint8>, key: seq<uint8>, msg: seq<uint8>, aad: seq<uint8>)
       returns (res : Result<EncryptionOutput>)
     requires encAlg.Valid()
     requires encAlg.alg.AES?
@@ -46,8 +50,12 @@ module {:extern "AESEncryption"} AESEncryption {
     ensures res.Success? ==>
       |res.value.cipherText| == |msg| && |res.value.authTag| == encAlg.tagLen as int
     ensures res.Success? ==> EncryptionOutputEncryptedWithAAD(res.value, aad)
-    ensures res.Success? ==> DecryptMock(res.value.cipherText) == msg
-    ensures res.Success? ==> res.value.cipherText == EncryptMock(msg)
+    ensures res.Success? ==> IsEncrypted(res.value.cipherText, msg)
+    {
+      res := AESEncrypt(encAlg, iv, key, msg, aad);
+      expect res.Success? ==> |res.value.cipherText| == |msg|;
+      expect res.Success? ==> |res.value.authTag| == encAlg.tagLen as int;
+    }
 
   method {:extern "AESEncryption.AES_GCM", "AESDecrypt"} AESDecrypt(encAlg: EncryptionSuites.EncryptionSuite, key: seq<uint8>, cipherTxt: seq<uint8>, authTag: seq<uint8>, iv: seq<uint8>, aad: seq<uint8>)
       returns (res: Result<seq<uint8>>)
@@ -58,7 +66,22 @@ module {:extern "AESEncryption"} AESEncryption {
     requires |iv| == encAlg.ivLen as int
     requires |authTag| == encAlg.tagLen as int
     ensures res.Success? ==> PlaintextDecryptedWithAAD(res.value, aad)
-    ensures res.Success? ==> DecryptMock(cipherTxt) == res.value
-    ensures res.Success? ==> cipherTxt == EncryptMock(res.value)
+    ensures res.Success? ==> IsEncrypted(cipherTxt, res.value) 
+
+  method AESDecryptWrapper(encAlg: EncryptionSuites.EncryptionSuite, key: seq<uint8>, cipherTxt: seq<uint8>, authTag: seq<uint8>, iv: seq<uint8>, aad: seq<uint8>)
+      returns (res: Result<seq<uint8>>)
+    requires encAlg.Valid()
+    requires encAlg.alg.AES?
+    requires encAlg.alg.mode.GCM?
+    requires |key| == encAlg.keyLen as int
+    requires |iv| == encAlg.ivLen as int
+    requires |authTag| == encAlg.tagLen as int
+    ensures res.Success? ==> |res.value| == |cipherTxt|
+    ensures res.Success? ==> PlaintextDecryptedWithAAD(res.value, aad)
+    ensures res.Success? ==> IsEncrypted(cipherTxt, res.value)
+    {
+      res := AESDecrypt(encAlg, key, cipherTxt, authTag, iv, aad);
+      expect res.Success? ==> |cipherTxt| == |res.value|;
+    }
 
 }
